new/golang/theory/proofmode.v
@@ -72,7 +72,8 @@ End classes.
 
 (** Some basic, primitive instances. Adapted to use `IntoVal`. *)
 Section instances.
-Context `{ffi_sem: ffi_semantics} `{!ffi_interp ffi} `{!gooseGlobalGS Σ, !gooseLocalGS Σ}.
+Context `{ffi_sem: ffi_semantics} `{!ffi_interp ffi} `{!gooseGlobalGS Σ, !gooseLocalGS Σ}
+         {core_sem : go.CoreSemantics}.
 
 Global Instance wp_injl (v : val) : PureWp True (InjL v) (InjLV v).
 Proof. apply (pure_exec_pure_wp O). solve_pure_exec. Qed.
@@ -87,16 +88,16 @@ Global Instance wp_fst (v1 v2 : val) : PureWp True (Fst (v1, v2)%V) v1.
 Proof. apply (pure_exec_pure_wp O). solve_pure_exec. Qed.
 
 Global Instance wp_recc f x erec : PureWp True (rec: f x := erec)%E #(func.mk f x erec).
-Proof. rewrite into_val_unseal. apply (pure_exec_pure_wp O). solve_pure_exec. Qed.
+Proof. rewrite !go.into_val_unfold. apply (pure_exec_pure_wp O). solve_pure_exec. Qed.
 
 Global Instance wp_pair (v1 v2 : val) : PureWp True (v1, v2)%E (v1, v2)%V.
 Proof. apply (pure_exec_pure_wp O). solve_pure_exec. Qed.
 
 Global Instance wp_if_false e1 e2 : PureWp True (if: #false then e1 else e2) e2.
-Proof. apply (pure_exec_pure_wp O). rewrite into_val_unseal. solve_pure_exec. Qed.
+Proof. apply (pure_exec_pure_wp O). rewrite !go.into_val_unfold. solve_pure_exec. Qed.
 
 Global Instance wp_if_true e1 e2 : PureWp True (if: #true then e1 else e2) e1.
-Proof. apply (pure_exec_pure_wp O). rewrite into_val_unseal. solve_pure_exec. Qed.
+Proof. apply (pure_exec_pure_wp O). rewrite !go.into_val_unfold. solve_pure_exec. Qed.
 
 Global Instance wp_case_inr v e1 e2 : PureWp True (Case (InjRV v) e1 e2) (e2 v).
 Proof. apply (pure_exec_pure_wp O). solve_pure_exec. Qed.
@@ -110,7 +111,7 @@ Proof.
   apply (pure_exec_pure_wp O).
   intros Hcomp.
   cut (bin_op_eval EqOp v1 v2 = Some $ LitV $ LitBool $ bool_decide (v1 = v2)).
-  { rewrite into_val_unseal. solve_pure_exec. }
+  { rewrite !go.into_val_unfold. solve_pure_exec. }
   rewrite /bin_op_eval /bin_op_eval_eq /=.
   rewrite decide_True //.
 Qed.
@@ -118,142 +119,142 @@ Qed.
 (** Unops *)
 (* w64 unops *)
 Global Instance wp_neg_w64 (v : w64) : PureWp True (~#v) #(word.not v).
-Proof. rewrite into_val_unseal. apply (pure_exec_pure_wp O). solve_pure_exec. Qed.
+Proof. rewrite !go.into_val_unfold. apply (pure_exec_pure_wp O). solve_pure_exec. Qed.
 
 Global Instance wp_w64_u_to_w64 (v : w64) : PureWp True (u_to_w64 #v) #v.
 Proof.
-  rewrite into_val_unseal. apply (pure_exec_pure_wp O).
+  rewrite !go.into_val_unfold. apply (pure_exec_pure_wp O).
   solve_pure_exec. replace (_ (uint.Z v)) with v by word. done.
 Qed.
 
 Global Instance wp_w64_u_to_w32 (v : w64) : PureWp True (u_to_w32 #v) #(W32 $ uint.Z v).
-Proof. rewrite into_val_unseal. apply (pure_exec_pure_wp O). solve_pure_exec. Qed.
+Proof. rewrite !go.into_val_unfold. apply (pure_exec_pure_wp O). solve_pure_exec. Qed.
 
 Global Instance wp_w64_u_to_w16 (v : w64) : PureWp True (u_to_w16 #v) #(W16 $ uint.Z v).
-Proof. rewrite into_val_unseal. apply (pure_exec_pure_wp O). solve_pure_exec. Qed.
+Proof. rewrite !go.into_val_unfold. apply (pure_exec_pure_wp O). solve_pure_exec. Qed.
 
 Global Instance wp_w64_u_to_w8 (v : w64) : PureWp True (u_to_w8 #v) #(W8 $ uint.Z v).
-Proof. rewrite into_val_unseal. apply (pure_exec_pure_wp O). solve_pure_exec. Qed.
+Proof. rewrite !go.into_val_unfold. apply (pure_exec_pure_wp O). solve_pure_exec. Qed.
 
 Global Instance wp_w64_s_to_w64 (v : w64) : PureWp True (s_to_w64 #v) #v.
 Proof.
-  rewrite into_val_unseal. apply (pure_exec_pure_wp O).
+  rewrite !go.into_val_unfold. apply (pure_exec_pure_wp O).
   solve_pure_exec. replace (_ (sint.Z v)) with v by word. done.
 Qed.
 
 Global Instance wp_w64_s_to_w32 (v : w64) : PureWp True (s_to_w32 #v) #(W32 $ sint.Z v).
-Proof. rewrite into_val_unseal. apply (pure_exec_pure_wp O). solve_pure_exec. Qed.
+Proof. rewrite !go.into_val_unfold. apply (pure_exec_pure_wp O). solve_pure_exec. Qed.
 
 Global Instance wp_w64_s_to_w16 (v : w64) : PureWp True (s_to_w16 #v) #(W16 $ sint.Z v).
-Proof. rewrite into_val_unseal. apply (pure_exec_pure_wp O). solve_pure_exec. Qed.
+Proof. rewrite !go.into_val_unfold. apply (pure_exec_pure_wp O). solve_pure_exec. Qed.
 
 Global Instance wp_w64_s_to_w8 (v : w64) : PureWp True (s_to_w8 #v) #(W8 $ sint.Z v).
-Proof. rewrite into_val_unseal. apply (pure_exec_pure_wp O). solve_pure_exec. Qed.
+Proof. rewrite !go.into_val_unfold. apply (pure_exec_pure_wp O). solve_pure_exec. Qed.
 
 (* w32 unops *)
 Global Instance wp_neg_w32 (v : w32) : PureWp True (~#v) #(word.not v).
-Proof. rewrite into_val_unseal. apply (pure_exec_pure_wp O). solve_pure_exec. Qed.
+Proof. rewrite !go.into_val_unfold. apply (pure_exec_pure_wp O). solve_pure_exec. Qed.
 
 Global Instance wp_w32_u_to_w64 (v : w32) : PureWp True (u_to_w64 #v) #(W64 $ uint.Z v).
-Proof. rewrite into_val_unseal. apply (pure_exec_pure_wp O). solve_pure_exec. Qed.
+Proof. rewrite !go.into_val_unfold. apply (pure_exec_pure_wp O). solve_pure_exec. Qed.
 
 Global Instance wp_w32_u_to_w32 (v : w32) : PureWp True (u_to_w32 #v) #v.
 Proof.
-  rewrite into_val_unseal. apply (pure_exec_pure_wp O).
+  rewrite !go.into_val_unfold. apply (pure_exec_pure_wp O).
   solve_pure_exec. replace (_ (uint.Z v)) with v by word. done.
 Qed.
 
 Global Instance wp_w32_u_to_w16 (v : w32) : PureWp True (u_to_w16 #v) #(W16 $ uint.Z v).
-Proof. rewrite into_val_unseal. apply (pure_exec_pure_wp O). solve_pure_exec. Qed.
+Proof. rewrite !go.into_val_unfold. apply (pure_exec_pure_wp O). solve_pure_exec. Qed.
 
 Global Instance wp_w32_u_to_w8 (v : w32) : PureWp True (u_to_w8 #v) #(W8 $ uint.Z v).
-Proof. rewrite into_val_unseal. apply (pure_exec_pure_wp O). solve_pure_exec. Qed.
+Proof. rewrite !go.into_val_unfold. apply (pure_exec_pure_wp O). solve_pure_exec. Qed.
 
 Global Instance wp_w32_s_to_w64 (v : w32) : PureWp True (s_to_w64 #v) #(W64 $ sint.Z v).
-Proof. rewrite into_val_unseal. apply (pure_exec_pure_wp O). solve_pure_exec. Qed.
+Proof. rewrite !go.into_val_unfold. apply (pure_exec_pure_wp O). solve_pure_exec. Qed.
 
 Global Instance wp_w32_s_to_w32 (v : w32) : PureWp True (s_to_w32 #v) #v.
 Proof.
-  rewrite into_val_unseal. apply (pure_exec_pure_wp O).
+  rewrite !go.into_val_unfold. apply (pure_exec_pure_wp O).
   solve_pure_exec. replace (_ (sint.Z v)) with v by word. done.
 Qed.
 
 Global Instance wp_w32_s_to_w16 (v : w32) : PureWp True (s_to_w16 #v) #(W16 $ sint.Z v).
-Proof. rewrite into_val_unseal. apply (pure_exec_pure_wp O). solve_pure_exec. Qed.
+Proof. rewrite !go.into_val_unfold. apply (pure_exec_pure_wp O). solve_pure_exec. Qed.
 
 Global Instance wp_w32_s_to_w8 (v : w32) : PureWp True (s_to_w8 #v) #(W8 $ sint.Z v).
-Proof. rewrite into_val_unseal. apply (pure_exec_pure_wp O). solve_pure_exec. Qed.
+Proof. rewrite !go.into_val_unfold. apply (pure_exec_pure_wp O). solve_pure_exec. Qed.
 
 (* w8 unops *)
 Global Instance wp_neg_w8 (v : w8) : PureWp True (~#v) #(word.not v).
-Proof. rewrite into_val_unseal. apply (pure_exec_pure_wp O). solve_pure_exec. Qed.
+Proof. rewrite !go.into_val_unfold. apply (pure_exec_pure_wp O). solve_pure_exec. Qed.
 
 Global Instance wp_w8_u_to_w64 (v : w8) : PureWp True (u_to_w64 #v) #(W64 $ uint.Z v).
-Proof. rewrite into_val_unseal. apply (pure_exec_pure_wp O). solve_pure_exec. Qed.
+Proof. rewrite !go.into_val_unfold. apply (pure_exec_pure_wp O). solve_pure_exec. Qed.
 
 Global Instance wp_w8_u_to_w32 (v : w8) : PureWp True (u_to_w32 #v) #(W32 $ uint.Z v).
-Proof. rewrite into_val_unseal. apply (pure_exec_pure_wp O). solve_pure_exec. Qed.
+Proof. rewrite !go.into_val_unfold. apply (pure_exec_pure_wp O). solve_pure_exec. Qed.
 
 Global Instance wp_w8_u_to_w8 (v : w8) : PureWp True (u_to_w8 #v) #v.
 Proof.
-  rewrite into_val_unseal. apply (pure_exec_pure_wp O).
+  rewrite !go.into_val_unfold. apply (pure_exec_pure_wp O).
   solve_pure_exec. replace (_ (uint.Z v)) with v by word. done.
 Qed.
 
 Global Instance wp_w8_s_to_w64 (v : w8) : PureWp True (s_to_w64 #v) #(W64 $ sint.Z v).
-Proof. rewrite into_val_unseal. apply (pure_exec_pure_wp O). solve_pure_exec. Qed.
+Proof. rewrite !go.into_val_unfold. apply (pure_exec_pure_wp O). solve_pure_exec. Qed.
 
 Global Instance wp_w8_s_to_w32 (v : w8) : PureWp True (s_to_w32 #v) #(W32 $ sint.Z v).
-Proof. rewrite into_val_unseal. apply (pure_exec_pure_wp O). solve_pure_exec. Qed.
+Proof. rewrite !go.into_val_unfold. apply (pure_exec_pure_wp O). solve_pure_exec. Qed.
 
 Global Instance wp_w8_s_to_w8 (v : w8) : PureWp True (s_to_w8 #v) #v.
 Proof.
-  rewrite into_val_unseal. apply (pure_exec_pure_wp O).
+  rewrite !go.into_val_unfold. apply (pure_exec_pure_wp O).
   solve_pure_exec. replace (_ (sint.Z v)) with v by word. done.
 Qed.
 
 Global Instance wp_w8_to_string (v : w8) : PureWp True (to_string #v) #([v]).
-Proof. rewrite into_val_unseal. apply (pure_exec_pure_wp O). solve_pure_exec. Qed.
+Proof. rewrite !go.into_val_unfold. apply (pure_exec_pure_wp O). solve_pure_exec. Qed.
 
 (* w16 unops *)
 Global Instance wp_neg_w16 (v : w16) : PureWp True (~#v) #(word.not v).
-Proof. rewrite into_val_unseal. apply (pure_exec_pure_wp O). solve_pure_exec. Qed.
+Proof. rewrite !go.into_val_unfold. apply (pure_exec_pure_wp O). solve_pure_exec. Qed.
 
 Global Instance wp_w16_u_to_w64 (v : w16) : PureWp True (u_to_w64 #v) #(W64 $ uint.Z v).
-Proof. rewrite into_val_unseal. apply (pure_exec_pure_wp O). solve_pure_exec. Qed.
+Proof. rewrite !go.into_val_unfold. apply (pure_exec_pure_wp O). solve_pure_exec. Qed.
 
 Global Instance wp_w16_u_to_w32 (v : w16) : PureWp True (u_to_w32 #v) #(W32 $ uint.Z v).
-Proof. rewrite into_val_unseal. apply (pure_exec_pure_wp O). solve_pure_exec. Qed.
+Proof. rewrite !go.into_val_unfold. apply (pure_exec_pure_wp O). solve_pure_exec. Qed.
 
 Global Instance wp_w16_u_to_w16 (v : w16) : PureWp True (u_to_w16 #v) #(W16 $ uint.Z v).
-Proof. rewrite into_val_unseal. apply (pure_exec_pure_wp O). solve_pure_exec. Qed.
+Proof. rewrite !go.into_val_unfold. apply (pure_exec_pure_wp O). solve_pure_exec. Qed.
 
 Global Instance wp_w16_u_to_w8 (v : w16) : PureWp True (u_to_w8 #v) #(W8 $ uint.Z v).
-Proof. rewrite into_val_unseal. apply (pure_exec_pure_wp O). solve_pure_exec. Qed.
+Proof. rewrite !go.into_val_unfold. apply (pure_exec_pure_wp O). solve_pure_exec. Qed.
 
 Global Instance wp_w16_s_to_w64 (v : w16) : PureWp True (s_to_w64 #v) #(W64 $ sint.Z v).
-Proof. rewrite into_val_unseal. apply (pure_exec_pure_wp O). solve_pure_exec. Qed.
+Proof. rewrite !go.into_val_unfold. apply (pure_exec_pure_wp O). solve_pure_exec. Qed.
 
 Global Instance wp_w16_s_to_w32 (v : w16) : PureWp True (s_to_w32 #v) #(W32 $ sint.Z v).
-Proof. rewrite into_val_unseal. apply (pure_exec_pure_wp O). solve_pure_exec. Qed.
+Proof. rewrite !go.into_val_unfold. apply (pure_exec_pure_wp O). solve_pure_exec. Qed.
 
 Global Instance wp_w16_s_to_w16 (v : w16) : PureWp True (s_to_w16 #v) #(W16 $ sint.Z v).
-Proof. rewrite into_val_unseal. apply (pure_exec_pure_wp O). solve_pure_exec. Qed.
+Proof. rewrite !go.into_val_unfold. apply (pure_exec_pure_wp O). solve_pure_exec. Qed.
 
 Global Instance wp_w16_s_to_w8 (v : w16) : PureWp True (s_to_w8 #v) #(W8 $ sint.Z v).
-Proof. rewrite into_val_unseal. apply (pure_exec_pure_wp O). solve_pure_exec. Qed.
+Proof. rewrite !go.into_val_unfold. apply (pure_exec_pure_wp O). solve_pure_exec. Qed.
 
 (* bool unop *)
 Global Instance wp_bool_neg (b : bool) : PureWp True (~ #b) #(Datatypes.negb b).
-Proof. rewrite into_val_unseal. apply (pure_exec_pure_wp O). solve_pure_exec. Qed.
+Proof. rewrite !go.into_val_unfold. apply (pure_exec_pure_wp O). solve_pure_exec. Qed.
 
 (* string unop *)
 Global Instance wp_StringLength (s : go_string) : PureWp True (StringLength #s) #(W64 $ length s).
-Proof. rewrite into_val_unseal. apply (pure_exec_pure_wp O). solve_pure_exec. Qed.
+Proof. rewrite !go.into_val_unfold. apply (pure_exec_pure_wp O). solve_pure_exec. Qed.
 
 Global Instance wp_IsNoStringOverflow (s : go_string) : PureWp True (IsNoStringOverflow #s)
                                                        #(bool_decide ((length s) < 2^64)).
-Proof. rewrite into_val_unseal. apply (pure_exec_pure_wp O). solve_pure_exec. Qed.
+Proof. rewrite !go.into_val_unfold. apply (pure_exec_pure_wp O). solve_pure_exec. Qed.
 
 (** Binops *)
 
@@ -263,9 +264,9 @@ Global Instance wp_w64_binop op (v1 v2 : w64) (v : val) :
       (into_val <$> bin_op_eval_word op v1 v2) ∪ (into_val <$> bin_op_eval_compare op v1 v2) = Some v)
     (BinOp op #v1 #v2)%E v | 1.
 Proof.
-  rewrite into_val_unseal /=. apply (pure_exec_pure_wp O).
+  apply (pure_exec_pure_wp O). rewrite !go.into_val_unfold /=.
   intros [??]. assert (bin_op_eval op (LitV v1) (LitV v2) = Some v).
-  { rewrite /bin_op_eval decide_False // /=. destruct op; try by simpl in *. }
+  { rewrite /bin_op_eval decide_False // /=. destruct op; by simpl in *. }
   revert H. solve_pure_exec.
 Qed.
 
@@ -274,7 +275,7 @@ Global Instance wp_w32_binop op (v1 v2 : w32) (v : val) :
       (into_val <$> bin_op_eval_word op v1 v2) ∪ (into_val <$> bin_op_eval_compare op v1 v2) = Some v)
     (BinOp op #v1 #v2)%E v | 1.
 Proof.
-  rewrite into_val_unseal /=. apply (pure_exec_pure_wp O).
+  rewrite !go.into_val_unfold /=. apply (pure_exec_pure_wp O).
   intros [??]. assert (bin_op_eval op (LitV v1) (LitV v2) = Some v).
   { rewrite /bin_op_eval decide_False // /=. destruct op; try by simpl in *. }
   revert H. solve_pure_exec.
@@ -285,7 +286,7 @@ Global Instance wp_w16_binop op (v1 v2 : w16) (v : val) :
       (into_val <$> bin_op_eval_word op v1 v2) ∪ (into_val <$> bin_op_eval_compare op v1 v2) = Some v)
     (BinOp op #v1 #v2)%E v | 1.
 Proof.
-  rewrite into_val_unseal /=. apply (pure_exec_pure_wp O).
+  rewrite !go.into_val_unfold /=. apply (pure_exec_pure_wp O).
   intros [??]. assert (bin_op_eval op (LitV v1) (LitV v2) = Some v).
   { rewrite /bin_op_eval decide_False // /=. destruct op; try by simpl in *. }
   revert H. solve_pure_exec.
@@ -296,7 +297,7 @@ Global Instance wp_w8_binop op (v1 v2 : w8) (v : val) :
       (into_val <$> bin_op_eval_word op v1 v2) ∪ (into_val <$> bin_op_eval_compare op v1 v2) = Some v)
     (BinOp op #v1 #v2)%E v | 1.
 Proof.
-  rewrite into_val_unseal /=. apply (pure_exec_pure_wp O).
+  rewrite !go.into_val_unfold /=. apply (pure_exec_pure_wp O).
   intros [??]. assert (bin_op_eval op (LitV v1) (LitV v2) = Some v).
   { rewrite /bin_op_eval decide_False // /=. destruct op; try by simpl in *. }
   revert H. solve_pure_exec.
@@ -305,7 +306,7 @@ Qed.
 Global Instance wp_w8_w64_binop op (v1 : w8) (v2 : w64) (v : w8) :
   PureWp (bin_op_eval_shift op v1 (W8 (uint.Z v2)) = Some v) (BinOp op #v1 #v2) #v | 1.
 Proof.
-  rewrite into_val_unseal. apply (pure_exec_pure_wp O).
+  rewrite !go.into_val_unfold. apply (pure_exec_pure_wp O).
   rewrite /bin_op_eval_shift /=.
   intros H. destruct op; simpl in H; try by exfalso.
   all: revert H; solve_pure_exec; inversion H; subst; done.
@@ -314,7 +315,7 @@ Qed.
 Global Instance wp_w8_w16_binop op (v1 : w8) (v2 : w16) (v : w8) :
   PureWp (bin_op_eval_shift op v1 (W8 (uint.Z v2)) = Some v) (BinOp op #v1 #v2) #v | 1.
 Proof.
-  rewrite into_val_unseal. apply (pure_exec_pure_wp O).
+  rewrite !go.into_val_unfold. apply (pure_exec_pure_wp O).
   intros H. destruct op; simpl in H; try by exfalso.
   all: revert H; solve_pure_exec; inversion H; subst; done.
 Qed.
@@ -322,7 +323,7 @@ Qed.
 Global Instance wp_w8_w32_binop op (v1 : w8) (v2 : w32) (v : w8) :
   PureWp (bin_op_eval_shift op v1 (W8 (uint.Z v2)) = Some v) (BinOp op #v1 #v2) #v | 1.
 Proof.
-  rewrite into_val_unseal. apply (pure_exec_pure_wp O).
+  rewrite !go.into_val_unfold. apply (pure_exec_pure_wp O).
   intros H. destruct op; simpl in H; try by exfalso.
   all: revert H; solve_pure_exec; inversion H; subst; done.
 Qed.
@@ -330,7 +331,7 @@ Qed.
 Global Instance wp_w32_w64_binop op (v1 : w32) (v2 : w64) (v : w32) :
   PureWp (bin_op_eval_shift op v1 (W32 (uint.Z v2)) = Some v) (BinOp op #v1 #v2) #v | 1.
 Proof.
-  rewrite into_val_unseal. apply (pure_exec_pure_wp O).
+  rewrite !go.into_val_unfold. apply (pure_exec_pure_wp O).
   intros H. destruct op; simpl in H; try by exfalso.
   all: revert H; solve_pure_exec; inversion H; subst; done.
 Qed.
@@ -338,7 +339,7 @@ Qed.
 Global Instance wp_w32_w16_binop op (v1 : w32) (v2 : w16) (v : w32) :
   PureWp (bin_op_eval_shift op v1 (W32 (uint.Z v2)) = Some v) (BinOp op #v1 #v2) #v | 1.
 Proof.
-  rewrite into_val_unseal. apply (pure_exec_pure_wp O).
+  rewrite !go.into_val_unfold. apply (pure_exec_pure_wp O).
   intros H. destruct op; simpl in H; try by exfalso.
   all: revert H; solve_pure_exec; inversion H; subst; done.
 Qed.
@@ -346,7 +347,7 @@ Qed.
 Global Instance wp_w32_w8_binop op (v1 : w32) (v2 : w8) (v : w32) :
   PureWp (bin_op_eval_shift op v1 (W32 (uint.Z v2)) = Some v) (BinOp op #v1 #v2) #v | 1.
 Proof.
-  rewrite into_val_unseal. apply (pure_exec_pure_wp O).
+  rewrite !go.into_val_unfold. apply (pure_exec_pure_wp O).
   intros H. destruct op; simpl in H; try by exfalso.
   all: revert H; solve_pure_exec; inversion H; subst; done.
 Qed.
@@ -354,7 +355,7 @@ Qed.
 Global Instance wp_w64_w16_binop op (v1 : w64) (v2 : w16) (v : w64) :
   PureWp (bin_op_eval_shift op v1 (W64 (uint.Z v2)) = Some v) (BinOp op #v1 #v2) #v | 1.
 Proof.
-  rewrite into_val_unseal. apply (pure_exec_pure_wp O).
+  rewrite !go.into_val_unfold. apply (pure_exec_pure_wp O).
   intros H. destruct op; simpl in H; try by exfalso.
   all: revert H; solve_pure_exec; inversion H; subst; done.
 Qed.
@@ -362,7 +363,7 @@ Qed.
 Global Instance wp_w64_w8_binop op (v1 : w64) (v2 : w8) (v : w64) :
   PureWp (bin_op_eval_shift op v1 (W64 (uint.Z v2)) = Some v) (BinOp op #v1 #v2) #v | 1.
 Proof.
-  rewrite into_val_unseal. apply (pure_exec_pure_wp O).
+  rewrite !go.into_val_unfold. apply (pure_exec_pure_wp O).
   intros H. destruct op; simpl in H; try by exfalso.
   all: revert H; solve_pure_exec; inversion H; subst; done.
 Qed.
@@ -370,7 +371,7 @@ Qed.
 Global Instance wp_w64_w32_binop op (v1 : w64) (v2 : w32) (v : w64) :
   PureWp (bin_op_eval_shift op v1 (W64 (uint.Z v2)) = Some v) (BinOp op #v1 #v2) #v | 1.
 Proof.
-  rewrite into_val_unseal. apply (pure_exec_pure_wp O).
+  rewrite !go.into_val_unfold. apply (pure_exec_pure_wp O).
   intros H. destruct op; simpl in H; try by exfalso.
   all: revert H; solve_pure_exec; inversion H; subst; done.
 Qed.
@@ -378,7 +379,7 @@ Qed.
 Global Instance wp_w16_w64_binop op (v1 : w16) (v2 : w64) (v : w16) :
   PureWp (bin_op_eval_shift op v1 (W16 (uint.Z v2)) = Some v) (BinOp op #v1 #v2) #v | 1.
 Proof.
-  rewrite into_val_unseal. apply (pure_exec_pure_wp O).
+  rewrite !go.into_val_unfold. apply (pure_exec_pure_wp O).
   intros H. destruct op; simpl in H; try by exfalso.
   all: revert H; solve_pure_exec; inversion H; subst; done.
 Qed.
@@ -386,7 +387,7 @@ Qed.
 Global Instance wp_w16_w32_binop op (v1 : w16) (v2 : w32) (v : w16) :
   PureWp (bin_op_eval_shift op v1 (W16 (uint.Z v2)) = Some v) (BinOp op #v1 #v2) #v | 1.
 Proof.
-  rewrite into_val_unseal. apply (pure_exec_pure_wp O).
+  rewrite !go.into_val_unfold. apply (pure_exec_pure_wp O).
   intros H. destruct op; simpl in H; try by exfalso.
   all: revert H; solve_pure_exec; inversion H; subst; done.
 Qed.
@@ -394,7 +395,7 @@ Qed.
 Global Instance wp_w16_w8_binop op (v1 : w16) (v2 : w8) (v : w16) :
   PureWp (bin_op_eval_shift op v1 (W16 (uint.Z v2)) = Some v) (BinOp op #v1 #v2) #v | 1.
 Proof.
-  rewrite into_val_unseal. apply (pure_exec_pure_wp O).
+  rewrite !go.into_val_unfold. apply (pure_exec_pure_wp O).
   intros H. destruct op; simpl in H; try by exfalso.
   all: revert H; solve_pure_exec; inversion H; subst; done.
 Qed.
@@ -403,7 +404,7 @@ Qed.
 Global Instance wp_bool_binop op (v1 v2 v : bool) :
   PureWp (op ≠ EqOp ∧ bin_op_eval_bool op v1 v2 = Some v) (BinOp op #v1 #v2) #v | 1.
 Proof.
-  rewrite into_val_unseal. apply (pure_exec_pure_wp O).
+  rewrite !go.into_val_unfold. apply (pure_exec_pure_wp O).
   case => ?. solve_pure_exec.
   - rewrite /bin_op_eval decide_False // b /=. Transitions.monad_simpl.
   - rewrite /bin_op_eval decide_False // b /= in H0. by Transitions.monad_inv.
@@ -412,48 +413,10 @@ Qed.
 Global Instance wp_string_binop op (v1 v2 v : go_string) :
   PureWp (op ≠ EqOp ∧ bin_op_eval_string op v1 v2 = Some v) (BinOp op #v1 #v2) #v | 1.
 Proof.
-  rewrite into_val_unseal. apply (pure_exec_pure_wp O).
+  rewrite !go.into_val_unfold. apply (pure_exec_pure_wp O).
   case => ?. solve_pure_exec.
   - rewrite /bin_op_eval decide_False // b /=. Transitions.monad_simpl.
   - rewrite /bin_op_eval decide_False // b /= in H0. by Transitions.monad_inv.
-Qed.
-
-Global Instance wp_offset k (l : loc) (off : w64) :
-  PureWp True (BinOp (OffsetOp k) #l #off) #(l +ₗ k * (uint.Z off)).
-Proof. rewrite into_val_unseal. apply (pure_exec_pure_wp O). solve_pure_exec. Qed.
-
-(* string lookup ops *)
-
-Global Instance wp_StringGet_w64 (s : go_string) (i : w64) (v : w8) :
-  PureWp (s !! uint.nat i = Some v) (StringGet #s #i) #v.
-Proof.
-  rewrite into_val_unseal. apply (pure_exec_pure_wp O). solve_pure_exec.
-  - rewrite /bin_op_eval /= H /=. Transitions.monad_simpl.
-  - rewrite /bin_op_eval /= H /= in H1. Transitions.monad_inv. done.
-Qed.
-
-Global Instance wp_StringGet_w32 (s : go_string) (i : w32) (v : w8) :
-  PureWp (s !! uint.nat i = Some v) (StringGet #s #i) #v.
-Proof.
-  rewrite into_val_unseal. apply (pure_exec_pure_wp O). solve_pure_exec.
-  - rewrite /bin_op_eval /= H /=. Transitions.monad_simpl.
-  - rewrite /bin_op_eval /= H /= in H1. Transitions.monad_inv. done.
-Qed.
-
-Global Instance wp_StringGet_w16 (s : go_string) (i : w16) (v : w8) :
-  PureWp (s !! uint.nat i = Some v) (StringGet #s #i) #v.
-Proof.
-  rewrite into_val_unseal. apply (pure_exec_pure_wp O). solve_pure_exec.
-  - rewrite /bin_op_eval /= H /=. Transitions.monad_simpl.
-  - rewrite /bin_op_eval /= H /= in H1. Transitions.monad_inv. done.
-Qed.
-
-Global Instance wp_StringGet_w8 (s : go_string) (i : w8) (v : w8) :
-  PureWp (s !! uint.nat i = Some v) (StringGet #s #i) #v.
-Proof.
-  rewrite into_val_unseal. apply (pure_exec_pure_wp O). solve_pure_exec.
-  - rewrite /bin_op_eval /= H /=. Transitions.monad_simpl.
-  - rewrite /bin_op_eval /= H /= in H1. Transitions.monad_inv. done.
 Qed.
 
 (* XXX: making this an instance results in this fact getting used even in places
@@ -466,7 +429,7 @@ Proof. apply (pure_exec_pure_wp O). solve_pure_exec. Qed.
 
 Global Instance wp_call_go_func (v2 : val) f x e :
   PureWp True (App #(func.mk f x e) v2) (subst' x v2 (subst' f #(func.mk f x e) e)).
-Proof. rewrite into_val_unseal /=. apply (pure_exec_pure_wp O). solve_pure_exec. Qed.
+Proof. rewrite !go.into_val_unfold /=. apply (pure_exec_pure_wp O). solve_pure_exec. Qed.
 
 End instances.
 
@@ -494,7 +457,8 @@ Proof.
   by iApply wp_call.
 Qed.
 
-Lemma tac_wp_call_go_func `{ffi_sem: ffi_semantics} `{!ffi_interp ffi} `{!gooseGlobalGS Σ, !gooseLocalGS Σ}
+Lemma tac_wp_call_go_func `{ffi_sem: ffi_semantics} `{!ffi_interp ffi}
+  `{!gooseGlobalGS Σ, !gooseLocalGS Σ} `{!go.CoreSemantics}
       K f x e v2 Δ Δ' s E Φ :
   MaybeIntoLaterNEnvs 1 Δ Δ' →
   envs_entails Δ' (WP (fill K (subst' x v2 (subst' f #(func.mk f x e) e))) @ s; E {{ Φ }}) →
